preservation.lean
@@ -1,136 +1,192 @@
 import .syntax .notations .logic .evaluation .vcgen
 
-lemma same_free_and_left {P P' Q: prop}: FV P' = FV P → (FV (P' && Q) = FV (P && Q)) :=
+lemma same_free_and_left {P P' Q: prop}: FV P' = FV P → (FV (P' ⋀ Q) = FV (P ⋀ Q)) :=
   assume free_P'_P: FV P' = FV P,
   set.eq_of_subset_of_subset (
     assume x,
-    assume : x ∈ FV (P' && Q),
+    assume : x ∈ FV (P' ⋀ Q),
     or.elim (free_in_prop.and.inv this) (
       assume : x ∈ FV P',
       have x ∈ FV P, from free_P'_P ▸ this,
-      show x ∈ FV (P && Q), from free_in_prop.and₁ this
+      show x ∈ FV (P ⋀ Q), from free_in_prop.and₁ this
     ) (
       assume : x ∈ FV Q,
-      show x ∈ FV (P && Q), from free_in_prop.and₂ this
+      show x ∈ FV (P ⋀ Q), from free_in_prop.and₂ this
     )
   ) (
     assume x,
-    assume : x ∈ FV (P && Q),
+    assume : x ∈ FV (P ⋀ Q),
     or.elim (free_in_prop.and.inv this) (
       assume : x ∈ FV P,
       have x ∈ FV P', from free_P'_P.symm ▸ this,
-      show x ∈ FV (P' && Q), from free_in_prop.and₁ this
+      show x ∈ FV (P' ⋀ Q), from free_in_prop.and₁ this
     ) (
       assume : x ∈ FV Q,
-      show x ∈ FV (P' && Q), from free_in_prop.and₂ this
+      show x ∈ FV (P' ⋀ Q), from free_in_prop.and₂ this
     )
   )
 
-lemma same_calls_and_left {P P' Q: prop}: calls P' = calls P → (calls (P' && Q) = calls (P && Q)) :=
-  assume calls_P'_P: calls P' = calls P,
+lemma same_calls_and_left {P P' Q: prop} {σ: env}:
+      calls_env σ P' = calls_env σ P → (calls_env σ (P' ⋀ Q) = calls_env σ (P ⋀ Q)) :=
+  assume calls_P'_P: calls_env σ P' = calls_env σ P,
   set.eq_of_subset_of_subset (
     assume c: calltrigger,
-    assume : c ∈ calls (P' && Q),
-    or.elim (has_call.and.inv this) (
-      assume : c ∈ calls P',
-      have c ∈ calls P, from calls_P'_P ▸ this,
-      show c ∈ calls (P && Q), from has_call.and₁ this
+    assume : c ∈ calls_env σ (P' ⋀ Q),
+    or.elim (has_call_env.and.inv this) (
+      assume : c ∈ calls_env σ P',
+      have c ∈ calls_env σ P, from calls_P'_P ▸ this,
+      show c ∈ calls_env σ (P ⋀ Q), from has_call_env.and₁ this
     )
     (
-      assume : c ∈ calls Q,
-      show c ∈ calls (P && Q), from has_call.and₂ this
+      assume : c ∈ calls_env σ Q,
+      show c ∈ calls_env σ (P ⋀ Q), from has_call_env.and₂ this
     )
   )
   (
     assume c: calltrigger,
-    assume : c ∈ calls (P && Q),
-    or.elim (has_call.and.inv this) (
-      assume : c ∈ calls P,
-      have c ∈ calls P', from calls_P'_P.symm ▸ this,
-      show c ∈ calls (P' && Q), from has_call.and₁ this
+    assume : c ∈ calls_env σ (P ⋀ Q),
+    or.elim (has_call_env.and.inv this) (
+      assume : c ∈ calls_env σ P,
+      have c ∈ calls_env σ P', from calls_P'_P.symm ▸ this,
+      show c ∈ calls_env σ (P' ⋀ Q), from has_call_env.and₁ this
     )
     (
-      assume : c ∈ calls Q,
-      show c ∈ calls (P' && Q), from has_call.and₂ this
+      assume : c ∈ calls_env σ Q,
+      show c ∈ calls_env σ (P' ⋀ Q), from has_call_env.and₂ this
     )
   )
 
-lemma same_quantifiers_and_left {P P' Q: prop}: quantifiers P' = quantifiers P → (quantifiers (P' && Q) = quantifiers (P && Q)) :=
-  assume quantifiers_P'_P: quantifiers P' = quantifiers P,
-  set.eq_of_subset_of_subset (
-    assume c: callquantifier,
-    assume : c ∈ quantifiers (P' && Q),
-    or.elim (has_quantifier.and.inv this) (
-      assume : c ∈ quantifiers P',
-      have c ∈ quantifiers P, from quantifiers_P'_P ▸ this,
-      show c ∈ quantifiers (P && Q), from has_quantifier.and₁ this
-    )
-    (
-      assume : c ∈ quantifiers Q,
-      show c ∈ quantifiers (P && Q), from has_quantifier.and₂ this
-    )
+lemma same_quantifiers_and_left {P P' Q: prop} {σ: env}:
+      qualifiers_dominate σ P' P → qualifiers_dominate σ (P' ⋀ Q) (P ⋀ Q) :=
+  assume P'_dominates_P: qualifiers_dominate σ P' P,
+  assume (t₁: term) (x:var) (Q₁: prop),
+  assume : callquantifier.mk t₁ x Q₁ ∈ quantifiers (P ⋀ Q),
+  or.elim (has_quantifier.and.inv this) (
+    assume : callquantifier.mk t₁ x Q₁ ∈ quantifiers P,
+    have ∃(t₂: term) (Q₂: prop), callquantifier.mk t₂ x Q₂ ∈ quantifiers P' ∧
+        ∀v: value, σ[x↦v] ⊨ vc.implies Q₂.instantiated Q₁.instantiated,
+    from P'_dominates_P t₁ x Q₁ this,
+    let ⟨t₂, Q₂, ⟨call_t₂_Q₂_in_P', Q₂_impl_Q₁⟩⟩ := this in
+    have callquantifier.mk t₂ x Q₂ ∈ quantifiers (P' ⋀ Q), from has_quantifier.and₁ call_t₂_Q₂_in_P',
+    show ∃(t₂: term) (Q₂: prop), callquantifier.mk t₂ x Q₂ ∈ quantifiers (P' ⋀ Q) ∧
+        ∀v: value, σ[x↦v] ⊨ vc.implies Q₂.instantiated Q₁.instantiated,
+    from exists.intro t₂ (exists.intro Q₂ ⟨this, Q₂_impl_Q₁⟩)
+  ) (
+    assume : callquantifier.mk t₁ x Q₁ ∈ quantifiers Q,
+    have h1: callquantifier.mk t₁ x Q₁ ∈ quantifiers (P' ⋀ Q), from has_quantifier.and₂ this,
+    have h2: ∀v: value, σ[x↦v] ⊨ vc.implies Q₁.instantiated Q₁.instantiated, from (
+      assume v: value,
+      show σ[x↦v] ⊨ vc.implies Q₁.instantiated Q₁.instantiated, from valid_env.mpr id
+    ),
+    show ∃(t₂: term) (Q₂: prop), callquantifier.mk t₂ x Q₂ ∈ quantifiers (P' ⋀ Q) ∧
+        ∀v: value, σ[x↦v] ⊨ vc.implies Q₂.instantiated Q₁.instantiated,
+    from exists.intro t₁ (exists.intro Q₁ ⟨h1, h2⟩)
   )
-  (
-    assume c: callquantifier,
-    assume : c ∈ quantifiers (P && Q),
-    or.elim (has_quantifier.and.inv this) (
-      assume : c ∈ quantifiers P,
-      have c ∈ quantifiers P', from quantifiers_P'_P.symm ▸ this,
-      show c ∈ quantifiers (P' && Q), from has_quantifier.and₁ this
-    )
-    (
-      assume : c ∈ quantifiers Q,
-      show c ∈ quantifiers (P' && Q), from has_quantifier.and₂ this
-    )
-  )
+
+lemma dominates_and_left {P P' Q: prop}:
+      (∀σ, dominates σ P' P) → (∀σ, dominates σ (P' ⋀ Q) (P ⋀ Q)) :=
+  assume h: ∀σ, dominates σ P' P,
+  assume σ: env,
+  have calls_env σ P' = calls_env σ P, from (h σ).left,
+  have h_calls: calls_env σ (P' ⋀ Q) = calls_env σ (P ⋀ Q), from same_calls_and_left this,
+  have qualifiers_dominate σ P' P, from (h σ).right.left,
+  have h_quantifiers: qualifiers_dominate σ (P' ⋀ Q) (P ⋀ Q), from same_quantifiers_and_left this,
+  have σ ⊨ vc.implies P'.instantiated_n P.instantiated_n, from (h σ).right.right,
+  have h_impl: σ ⊨ vc.implies (P' ⋀ Q).instantiated_n (P ⋀ Q).instantiated_n,
+  from valid_env.strengthen_and_with_dominating_instantiations (h σ),
+  ⟨h_calls, ⟨h_quantifiers, h_impl⟩⟩
 
 lemma strengthen_pre_exp {P: prop} {Q: propctx} {e: exp}:
-  (P ⊢ e : Q) →
-  ∀P': prop, (FV P' = FV P) → (calls P' = calls P) → (quantifiers P' = quantifiers P) →
-       (∀σ, σ ⊨ vc.implies P'.instantiated_n P.instantiated_n) →
-       (P' ⊢ e: Q) :=
+      (P ⊢ e : Q) → ∀P': prop, (FV P' = FV P) → (∀σ, dominates σ P' P) → (P' ⊢ e: Q) :=
   assume e_verified: (P ⊢ e : Q),
   begin
     induction e_verified,
     case exp.vcgen.tru x P e' Q x_not_free_in_P e'_verified ih { from (
       assume P': prop,
       assume free_P'_P: FV P' = FV P,
-      assume calls_P'_P: calls P' = calls P,
-      assume quantifiers_P'_P: quantifiers P' = quantifiers P,
-      assume strengthen_P'_P: (∀σ, σ ⊨ vc.implies P'.instantiated_n P.instantiated_n),
-      have h1: FV (P' && (x ≡ value.true)) = FV (P && (x ≡ value.true)),
+      assume P'_dominates_P: (∀σ, dominates σ P' P),
+
+      have h1: FV (P' ⋀ (x ≡ value.true)) = FV (P ⋀ (x ≡ value.true)),
       from same_free_and_left free_P'_P,
-      have h2: calls (P' && (x ≡ value.true)) = calls (P && (x ≡ value.true)),
-      from same_calls_and_left calls_P'_P,
-      have h3: quantifiers (P' && (x ≡ value.true)) = quantifiers (P && (x ≡ value.true)),
-      from same_quantifiers_and_left quantifiers_P'_P,
-      have h4: ∀σ, σ ⊨ vc.implies (P' && (x ≡ value.true)).instantiated_n (P && (x ≡ value.true)).instantiated_n,
-      from (assume σ, valid_env.strengthen_without_instantiations calls_P'_P quantifiers_P'_P (strengthen_P'_P σ)),
-      have e'_verified': P' && (x ≡ value.true) ⊢ e': Q,
-      from ih (P' && (x ≡ value.true)) h1 h2 h3 h4,
+      have h2: (∀σ, dominates σ (P' ⋀ (x ≡ value.true)) (P ⋀ (x ≡ value.true))),
+      from dominates_and_left P'_dominates_P,
+      have e'_verified': P' ⋀ (x ≡ value.true) ⊢ e': Q, from ih (P' ⋀ (x ≡ value.true)) h1 h2,
       have x_not_free_in_P': x ∉ FV P', from free_P'_P.symm ▸ x_not_free_in_P,
-      show P' ⊢ lett x = true in e' : propctx.exis x ((x ≡ value.true) && Q),
+      show P' ⊢ lett x = true in e' : propctx.exis x ((x ≡ value.true) ⋀ Q),
       from exp.vcgen.tru x_not_free_in_P' e'_verified'
     )},
     case exp.vcgen.fals x P e' Q x_not_free_in_P e'_verified ih { from
-
-    },
-    case exp.vcgen.num x n P e' Q x_not_free_in_P e'_verified ih { from
-
-    },
-    case exp.vcgen.func f x R S e₁ e₂ P Q₁ Q₂ f_not_free_in_P fv_R fv_S e₁_verified e₂_verified func_vc ih₁ ih₂ { from
       assume P': prop,
       assume free_P'_P: FV P' = FV P,
-      assume calls_P'_P: calls P' = calls P,
-      assume quantifiers_P'_P: quantifiers P' = quantifiers P,
-      assume strengthen_P'_P: (∀σ, σ ⊨ vc.implies P'.instantiated_n P.instantiated_n),
+      assume P'_dominates_P: (∀σ, dominates σ P' P),
 
+      have h1: FV (P' ⋀ (x ≡ value.false)) = FV (P ⋀ (x ≡ value.false)),
+      from same_free_and_left free_P'_P,
+      have h2: (∀σ, dominates σ (P' ⋀ (x ≡ value.false)) (P ⋀ (x ≡ value.false))),
+      from dominates_and_left P'_dominates_P,
+      have e'_verified': P' ⋀ (x ≡ value.false) ⊢ e': Q, from ih (P' ⋀ (x ≡ value.false)) h1 h2,
+      have x_not_free_in_P': x ∉ FV P', from free_P'_P.symm ▸ x_not_free_in_P,
+      show P' ⊢ letf x = false in e' : propctx.exis x ((x ≡ value.false) ⋀ Q),
+      from exp.vcgen.fals x_not_free_in_P' e'_verified'
+    },
+    case exp.vcgen.num x n P e' Q x_not_free_in_P e'_verified ih { from
+      assume P': prop,
+      assume free_P'_P: FV P' = FV P,
+      assume P'_dominates_P: (∀σ, dominates σ P' P),
+
+      have h1: FV (P' ⋀ (x ≡ value.num n)) = FV (P ⋀ (x ≡ value.num n)),
+      from same_free_and_left free_P'_P,
+      have h2: (∀σ, dominates σ (P' ⋀ (x ≡ value.num n)) (P ⋀ (x ≡ value.num n))),
+      from dominates_and_left P'_dominates_P,
+      have e'_verified': P' ⋀ (x ≡ value.num n) ⊢ e': Q, from ih (P' ⋀ (x ≡ value.num n)) h1 h2,
+      have x_not_free_in_P': x ∉ FV P', from free_P'_P.symm ▸ x_not_free_in_P,
+      show P' ⊢ letn x = n in e' : propctx.exis x ((x ≡ value.num n) ⋀ Q),
+      from exp.vcgen.num x_not_free_in_P' e'_verified'
+    },
+    case exp.vcgen.func f x R S e₁ e₂ P Q₁ Q₂ f_not_free_in_P x_not_free_in_P f_neq_x fv_R fv_S
+                        e₁_verified e₂_verified func_vc ih₁ ih₂ { from
+      assume P': prop,
+      assume free_P'_P: FV P' = FV P,
+      assume P'_dominates_P: (∀σ, dominates σ P' P),
 
       have f_not_free_in_P': f ∉ FV P', from free_P'_P.symm ▸ f_not_free_in_P,
+      have x_not_free_in_P': x ∉ FV P', from free_P'_P.symm ▸ x_not_free_in_P,
       have fv_R': FV R.to_prop ⊆ FV P' ∪ { f, x }, from free_P'_P.symm ▸ fv_R,
       have fv_S': FV S.to_prop ⊆ FV P' ∪ { f, x }, from free_P'_P.symm ▸ fv_S,
-      show P' ⊢ letf f[x] req R ens S {e₁} in e₂ : propctx.exis f (spec.func f x R S && Q₂),
-      from exp.vcgen.func f_not_free_in_P' fv_R' fv_S' 
+
+      have h1: FV (P' ⋀ ((spec.func f x R S) ⋀ R)) = FV (P ⋀ ((spec.func f x R S) ⋀ R)),
+      from same_free_and_left free_P'_P,
+      have h2: (∀σ, dominates σ (P' ⋀ (spec.func f x R S) ⋀ R) (P ⋀ (spec.func f x R S) ⋀ R)),
+      from dominates_and_left P'_dominates_P,
+      have e₁_verified': P' ⋀ (spec.func f x R S) ⋀ R ⊢ e₁ : Q₁,
+      from ih₁ (P' ⋀ (spec.func f x R S) ⋀ R) h1 h2,
+
+      have h3: FV (P' ⋀ (prop.func f x R (Q₁ (term.app ↑f ↑x) ⋀ ↑S)))
+             = FV (P ⋀ (prop.func f x R (Q₁ (term.app ↑f ↑x) ⋀ ↑S))),
+      from same_free_and_left free_P'_P,
+      have h4: (∀σ, dominates σ (P' ⋀ (prop.func f x R (Q₁ (term.app ↑f ↑x) ⋀ ↑S)))
+                                (P ⋀ (prop.func f x R (Q₁ (term.app ↑f ↑x) ⋀ ↑S)))),
+      from dominates_and_left P'_dominates_P,
+      have e₂_verified': P' ⋀ (prop.func f x R (Q₁ (term.app ↑f ↑x) ⋀ ↑S)) ⊢ e₂ : Q₂,
+      from ih₂ (P' ⋀ (prop.func f x R (Q₁ (term.app ↑f ↑x) ⋀ ↑S))) h3 h4,
+
+      have func_vc': ∀ (σ : env),
+             σ ⊨ prop.instantiated (prop.implies (P' ⋀ ↑(spec.func ↑f x R S) ⋀ R ⋀ Q₁ (term.app ↑f ↑x)) ↑S),
+      from (
+        assume σ: env,
+
+        have dominates σ (prop.or (P' ⋀ ↑(spec.func ↑f x R S) ⋀ R ⋀ Q₁ (term.app ↑f ↑x)).not
+        
+         ↑S).instantiated,
+
+
+        show σ ⊨ (prop.or (P' ⋀ ↑(spec.func ↑f x R S) ⋀ R ⋀ Q₁ (term.app ↑f ↑x)).not ↑S).instantiated,
+        from sorry
+      ),
+
+      show P' ⊢ letf f[x] req R ens S {e₁} in e₂ : propctx.exis f (prop.func f x R (Q₁ (term.app ↑f ↑x) ⋀ ↑S) ⋀ Q₂),
+      from exp.vcgen.func f_not_free_in_P' x_not_free_in_P' f_neq_x fv_R' fv_S' e₁_verified'
+           e₂_verified' func_vc'
     },
     case exp.vcgen.unop op x y e' Q' x_free_in_P _ e'_verified vc_valid { from
     },
