vcgen.lean
@@ -7,18 +7,18 @@ notation P `⊢` e `:` Q : 10 := exp.vcgen P e Q
 
 | tru {P: prop} {x: var} {e: exp} {Q: propctx}:
     x ∉ FV P →
-    (P && (x ≡ value.true) ⊢ e : Q) →
-    (P ⊢ lett x = true in e : propctx.exis x ((x ≡ value.true) && Q))
+    (P ⋀ x ≡ value.true ⊢ e : Q) →
+    (P ⊢ lett x = true in e : propctx.exis x (x ≡ value.true ⋀ Q))
 
 | fals {P: prop} {x: var} {e: exp} {Q: propctx}:
     x ∉ FV P →
-    (P && (x ≡ value.false) ⊢ e : Q) →
-    (P ⊢ letf x = false in e : propctx.exis x ((x ≡ value.false) && Q))
+    (P ⋀ x ≡ value.false ⊢ e : Q) →
+    (P ⊢ letf x = false in e : propctx.exis x (x ≡ value.false ⋀ Q))
 
 | num {P: prop} {x: var} {n: ℕ} {e: exp} {Q: propctx}:
     x ∉ FV P →
-    (P && (x ≡ value.num n) ⊢ e : Q) →
-    (P ⊢ letn x = n in e : propctx.exis x ((x ≡ value.num n) && Q))
+    (P ⋀ x ≡ value.num n ⊢ e : Q) →
+    (P ⊢ letn x = n in e : propctx.exis x (x ≡ value.num n ⋀ Q))
 
 | func {P: prop} {f x: var} {R S: spec} {e₁ e₂: exp} {Q₁ Q₂: propctx}:
     f ∉ FV P →
@@ -26,40 +26,40 @@ notation P `⊢` e `:` Q : 10 := exp.vcgen P e Q
     f ≠ x →
     FV R.to_prop ⊆ FV P ∪ { f, x } →
     FV S.to_prop ⊆ FV P ∪ { f, x } →
-    (P && spec.func f x R S && R ⊢ e₁ : Q₁) →
-    (P && prop.func f x R (Q₁ (term.app f x) && S) ⊢ e₂ : Q₂) →
-    ⟪prop.implies (P && spec.func f x R S && R && Q₁ (term.app f x)) S⟫ →
-    (P ⊢ letf f[x] req R ens S {e₁} in e₂ : propctx.exis f (prop.func f x R (Q₁ (term.app f x) && S) && Q₂))
+    (P ⋀ spec.func f x R S ⋀ R ⊢ e₁ : Q₁) →
+    (P ⋀ prop.func f x R (Q₁ (term.app f x) ⋀ S) ⊢ e₂ : Q₂) →
+    ⟪prop.implies (P ⋀ spec.func f x R S ⋀ R ⋀ Q₁ (term.app f x)) S⟫ →
+    (P ⊢ letf f[x] req R ens S {e₁} in e₂ : propctx.exis f (prop.func f x R (Q₁ (term.app f x) ⋀ S) ⋀ Q₂))
 
 | unop {P: prop} {op: unop} {e: exp} {x y: var} {Q: propctx}:
     x ∈ FV P →
     y ∉ FV P →
-    (P && (y ≡ term.unop op x) ⊢ e : Q) →
+    (P ⋀ y ≡ term.unop op x ⊢ e : Q) →
     ⟪ prop.implies P (prop.pre₁ op x) ⟫ →
-    (P ⊢ letop y = op [x] in e : propctx.exis y ((y ≡ term.unop op x) && Q))
+    (P ⊢ letop y = op [x] in e : propctx.exis y (y ≡ term.unop op x ⋀ Q))
 
 | binop {P: prop} {op: binop} {e: exp} {x y z: var} {Q: propctx}:
     x ∈ FV P →
     y ∈ FV P →
     z ∉ FV P →
-    (P && (z ≡ term.binop op x y) ⊢ e : Q) →
+    (P ⋀ z ≡ term.binop op x y ⊢ e : Q) →
     ⟪ prop.implies P (prop.pre₂ op x y) ⟫ →
-    (P ⊢ letop2 z = op [x, y] in e : propctx.exis z ((z ≡ term.binop op x y) && Q))
+    (P ⊢ letop2 z = op [x, y] in e : propctx.exis z (z ≡ term.binop op x y ⋀ Q))
 
 | app {P: prop} {e: exp} {y f x: var} {Q: propctx}:
     f ∈ FV P →
     x ∈ FV P →
     y ∉ FV P →
-    (P && prop.call f x && prop.post f x && (y ≡ term.app f x) ⊢ e : Q) →
-    ⟪ prop.implies (P && prop.call f x) (term.unop unop.isFunc f && prop.pre f x) ⟫ →
-    (P ⊢ letapp y = f [x] in e : propctx.exis y (prop.call f x && prop.post f x && (y ≡ term.app f x) && Q))
+    (P ⋀ prop.call f x ⋀ prop.post f x ⋀ y ≡ term.app f x ⊢ e : Q) →
+    ⟪ prop.implies (P ⋀ prop.call f x) (term.unop unop.isFunc f ⋀ prop.pre f x) ⟫ →
+    (P ⊢ letapp y = f [x] in e : propctx.exis y (prop.call f x ⋀ prop.post f x ⋀ y ≡ term.app f x ⋀ Q))
 
 | ite {P: prop} {e₁ e₂: exp} {x: var} {Q₁ Q₂: propctx}:
     x ∈ FV P →
-    (P && x ⊢ e₁ : Q₁) →
-    (P && term.unop unop.not x ⊢ e₂ : Q₂) →
+    (P ⋀ x ⊢ e₁ : Q₁) →
+    (P ⋀ term.unop unop.not x ⊢ e₂ : Q₂) →
     ⟪ prop.implies P (term.unop unop.isBool x) ⟫ →
-    (P ⊢ exp.ite x e₁ e₂ : (propctx.implies x Q₁ && propctx.implies (term.unop unop.not x) Q₂))
+    (P ⊢ exp.ite x e₁ e₂ : propctx.implies x Q₁ ⋀ propctx.implies (term.unop unop.not x) Q₂)
 
 | return {P: prop} {x: var}:
     x ∈ FV P →
@@ -76,17 +76,17 @@ notation `⊢` σ `:` Q : 10 := env.vcgen σ Q
 | tru {σ: env} {x: var} {Q: prop}:
     x ∉ σ →
     (⊢ σ : Q) →
-    (⊢ (σ[x ↦ value.true]) : (Q && (x ≡ value.true)))
+    (⊢ (σ[x ↦ value.true]) : Q ⋀ x ≡ value.true)
 
 | fls {σ: env} {x: var} {Q: prop}:
     x ∉ σ →
     (⊢ σ : Q) →
-    (⊢ (σ[x ↦ value.false]) : (Q && (x ≡ value.false)))
+    (⊢ (σ[x ↦ value.false]) : Q ⋀ x ≡ value.false)
 
 | num {n: ℤ} {σ: env} {x: var} {Q: prop}:
     x ∉ σ →
     (⊢ σ : Q) →
-    (⊢ (σ[x ↦ value.num n]) : (Q && (x ≡ value.num n)))
+    (⊢ (σ[x ↦ value.num n]) : Q ⋀ x ≡ value.num n)
 
 | func {σ₁ σ₂: env} {f g x: var} {R S: spec} {e: exp} {Q₁ Q₂: prop} {Q₃: propctx}:
     f ∉ σ₁ →
@@ -97,12 +97,12 @@ notation `⊢` σ `:` Q : 10 := env.vcgen σ Q
     (⊢ σ₂ : Q₂) →
     FV R.to_prop ⊆ FV Q₂ ∪ { g, x } →
     FV S.to_prop ⊆ FV Q₂ ∪ { g, x } →
-    (Q₂ && spec.func g x R S && R ⊢ e : Q₃) →
-    ⟪prop.implies (Q₂ && spec.func g x R S && R && Q₃ (term.app g x)) S⟫ →
+    (Q₂ ⋀ spec.func g x R S ⋀ R ⊢ e : Q₃) →
+    ⟪prop.implies (Q₂ ⋀ spec.func g x R S ⋀ R ⋀ Q₃ (term.app g x)) S⟫ →
     (⊢ (σ₁[f ↦ value.func g x R S e σ₂]) :
       (Q₁
-       && (f ≡ value.func g x R S e σ₂)
-       && prop.subst_env (σ₂[g↦value.func g x R S e σ₂]) (prop.func g x R (Q₃ (term.app g x) && S))))
+       ⋀ f ≡ value.func g x R S e σ₂
+       ⋀ prop.subst_env (σ₂[g↦value.func g x R S e σ₂]) (prop.func g x R (Q₃ (term.app g x) ⋀ S))))
 
 notation `⊢` σ `:` Q : 10 := env.vcgen σ Q
 
@@ -111,7 +111,7 @@ notation H `⊢ₛ` s : 10 := stack.vcgen H s
 
 | top {H: callhistory} {P: prop} {σ: env} {e: exp} {Q: propctx}:
     (⊢ σ : P) →
-    (H && P ⊢ e : Q) →
+    (H ⋀ P ⊢ e : Q) →
     (H ⊢ₛ (σ, e))
 
 | cons {H: callhistory} {P: prop} {s: stack} {σ₁ σ₂: env} {f fx g x y: var} {R S: spec} {e: exp} {v: value} {Q: propctx}:
@@ -120,8 +120,8 @@ notation H `⊢ₛ` s : 10 := stack.vcgen H s
     (σ₁ g = value.func f fx R S e σ₂) →
     (σ₁ x = v) →
     y ∉ σ₁ →
-    (H && P && prop.call g x && prop.post g x && (y ≡ term.app g x) ⊢ e : Q) →
-    ⟪ prop.implies (H && P && prop.call g x) (term.unop unop.isFunc g && prop.pre g x) ⟫ →
+    (H ⋀ P ⋀ prop.call g x ⋀ prop.post g x ⋀ y ≡ term.app g x ⊢ e : Q) →
+    ⟪ prop.implies (H ⋀ P ⋀ prop.call g x) (term.unop unop.isFunc g ⋀ prop.pre g x) ⟫ →
     ((σ₂[f↦value.func f fx R S e σ₂][fx↦v], e) ⟶* s) →
     (H ⊢ₛ (s · [σ₁, let y = g[x] in e]))
 
@@ -138,11 +138,11 @@ lemma exp.vcgen.return.inv {P: prop} {x: var} {Q: propctx}: (P ⊢ exp.return x 
     }
   end
 
-lemma stack.vcgen.top.inv {H: callhistory} {σ: env} {e: exp}: (H ⊢ₛ (σ, e)) → ∃P Q, (⊢ σ: P) ∧ (H && P ⊢ e: Q) :=
+lemma stack.vcgen.top.inv {H: callhistory} {σ: env} {e: exp}: (H ⊢ₛ (σ, e)) → ∃P Q, (⊢ σ: P) ∧ (H ⋀ P ⊢ e: Q) :=
   assume top_verified: H ⊢ₛ (σ, e),
   begin
     cases top_verified,
     case stack.vcgen.top P Q env_verified e_verified {
-      show ∃P Q, (⊢ σ: P) ∧ (H && P ⊢ e: Q), from exists.intro P (exists.intro Q ⟨env_verified, e_verified⟩)
+      show ∃P Q, (⊢ σ: P) ∧ (H ⋀ P ⊢ e: Q), from exists.intro P (exists.intro Q ⟨env_verified, e_verified⟩)
     }
   end
